update logrel_prim

theories/logrel/logrel_prim.v
@@ -47,88 +47,67 @@ Section slice.
   Context (i : VMID).
   Context `{vmG: !gen_VMG Σ}.
   Context (Φ_t : (gmap Addr transaction) -> VMID -> VMID -> iProp Σ).
-  Context (Φ_r : VMID -> VMID -> VMID -> iProp Σ).
-
-  Definition rx_state_none i : iProp Σ := RX_state@i := None ∗ ∃p_rx, RX@ i := p_rx ∗ (∃ mem_rx, memory_page p_rx mem_rx).
-
-  Definition rx_state_some i s : iProp Σ := RX_state{1/2}@i := Some(s).
-
-  Definition rx_state_match i os : iProp Σ :=
-    match os with
-                           | None => rx_state_none i
-                           | Some s => rx_state_some i s
-                          end.
-
-  Definition rx_states_global (rxs: gmap VMID (option (Word*VMID))) : iProp Σ :=
-    [∗ map]i ↦ os ∈ rxs, rx_state_match i os.
+  Context (Φ_r : VMID -> option (Word * VMID)-> VMID -> iProp Σ).
 
   Definition rx_states_transferred (rxs: gmap VMID (option (Word*VMID))) : iProp Σ :=
     [∗ map]i ↦ os ∈ rxs, match os with
                            | None => True
-                           | Some s => Φ_r i s.2 V0
+                           | Some s => Φ_r i os V0
                           end.
 
   Definition rx_states_owned (rxs: gmap VMID (option (Word*VMID))) : iProp Σ :=
     [∗ map]i ↦ os ∈ rxs, match os with
                            | None => True
-                           | Some s => if bool_decide (s.2 = V0) then Φ_r i V0 i else True
+                           | Some s => if bool_decide (s.2 = V0) then Φ_r i os i else True
                           end.
 
-  (* Definition rx_state_run (i j : VMID) rx_state : iProp Σ := *)
-  (*    (∃ p_rx, RX@ j := p_rx ∗  RX_state{1/2}@j := rx_state ∗ *)
-  (*                 match rx_state with *)
-  (*                 | None => (RX_state{1/2}@j := rx_state ∗ ∃ mem_rx, memory_page p_rx mem_rx) *)
-  (*                 | Some (_,v) => if bool_decide(i = j) then Φ_r v j else True *)
-  (*                 end)%I. *)
+  Definition return_reg_rx i (rs : option (Word * VMID)) (rxs :gmap VMID (option(Word*VMID))): iProp Σ:=
+    ((R0 @@ V0 ->r encode_hvc_func(Yield) ∨
+      R0 @@ V0 ->r encode_hvc_func(Wait) ∗ ⌜rs = None⌝)
+     ∗ rx_states_global (delete i rxs)
+     ∗ R1 @@ V0 ->r encode_vmid(i) ∗ ∃ r2, R2 @@ V0 ->r r2) ∨
+    (R0 @@ V0 ->r encode_hvc_func(Send)
+      ∗ ∃ l j, Φ_r j (Some (l,i)) V0
+      ∗ rx_states_global (<[j:=Some(l,i)]>(delete i rxs))
+      ∗ (∃r1, R1 @@ V0 ->r r1 ∗ ⌜decode_vmid r1 = Some j⌝) ∗  R2 @@ V0 ->r l).
 
-  Definition return_reg_rx i (rxs: gmap VMID (option (Word*VMID))): iProp Σ:=
-    ((R0 @@ V0 ->r encode_hvc_func(Yield) ∗ (∃ rx_state'', rx_state_match i rx_state'') ∨
-      R0 @@ V0 ->r encode_hvc_func(Wait) ∗ rx_state_match i None) ∗ R1 @@ V0 ->r encode_vmid(i) ∗ ∃ r2, R2 @@ V0 ->r r2) ∨
-    (R0 @@ V0 ->r encode_hvc_func(Send) ∗ (∃ rx_state'', rx_state_match i rx_state'') ∗ ∃ j l, ⌜j ≠ i⌝ ∗
-                          (∃r1, R1 @@ V0 ->r r1 ∗ ⌜decode_vmid r1 = Some j⌝) ∗  R2 @@ V0 ->r l ∗
-                              (Φ_r j i V0)).
-
-  Definition vmprop_zero_pre (Ψ: PID -d> PID -d> iPropO Σ) :PID -d> PID -d> (gmap VMID option(Word * VMID)) -d> iPropO Σ :=
-    λ p_tx p_rx, (∃ trans' rxs',
+  Definition vmprop_zero_pre (Ψ: PID -d> PID -d> iPropO Σ) :PID -d> PID -d> (gmap VMID (option(Word * VMID))) -d> iPropO Σ :=
+    λ p_tx p_rx rxs', (∃ trans' rs',
                            (* transaction and pagetable entries *)
                            transaction_hpool_global_transferred trans' ∗
                            big_sepSS_singleton set_of_vmids i (Φ_t trans') ∗
                            (* RX *)
                            rx_page i p_rx ∗
+                           rx_state_match i rs' ∗ Φ_r i rs' V0 ∗
                            rx_states_global (delete i rxs') ∗
-                           return_reg_rx i rxs' ∗
+                           return_reg_rx i rs' rxs' ∗
                            VMProp i (Ψ p_tx p_rx) (1/2)%Qp)%I.
 
   Definition vmprop_unknown_pre
     (Ψ : PID -d> PID -d> iPropO Σ)
     :PID -d> PID -d> iPropO Σ :=
-    λ p_tx p_rx,
-    (∃ (trans' : gmap Word transaction) rxs',
+    λ p_tx p_rx, (∃ (trans' : gmap Word transaction) (rxs : gmap VMID (option(Word * VMID))),
                (* transaction and pagetable entries *)
                transaction_hpool_global_transferred trans' ∗
                big_sepSS_singleton set_of_vmids i (Φ_t trans') ∗
                R0 @@ V0 ->r encode_hvc_func(Run) ∗ R1 @@ V0 ->r encode_vmid(i) ∗ (∃ r2, R2 @@ V0 ->r r2) ∗
                (* RX *)
                (rx_page i p_rx) ∗
-               (∃ rx_state', rx_state_match i rx_state' ∗
-               match rx_state' with
-               | None => True
-               | Some s => Φ_r i s.2 i
-               end) ∗ (* rx.state'.2 ≠ i *)
+               (∀ rs : option (Addr * VMID), ⌜rxs !! i = Some rs⌝ -∗ rx_state_match i rs ∗ Φ_r i rs i) ∗
                (* rx pages for all other VMs *)
-               (rx_states_global (delete i rxs')) ∗
+               (rx_states_global (delete i rxs)) ∗ ⌜is_total_gmap rxs⌝ ∗
                (* if i yielding, we give following resources back to pvm *)
-               VMProp V0 (vmprop_zero_pre Ψ p_tx p_rx) (1/2)%Qp)%I.
+               VMProp V0 (vmprop_zero_pre Ψ p_tx p_rx rxs) (1/2)%Qp)%I.
 
   Local Instance vmprop_unknown_pre_contractive : Contractive (vmprop_unknown_pre).
   Proof.
     rewrite /vmprop_unknown_pre => n vmprop_unknown vmprop_unknown' Hvmprop_unknown p_tx p_rx /=.
-    do 12 f_equiv.
+    do 13 f_equiv.
     rewrite /VMProp /=.
     do 6 f_equiv.
     f_contractive.
     rewrite /vmprop_zero_pre.
-    do 9 f_equiv.
+    do 11 f_equiv.
     rewrite /VMProp.
     repeat f_equiv.
   Qed.
@@ -138,20 +117,18 @@ Section slice.
   Definition vmprop_zero := vmprop_zero_pre vmprop_unknown.
 
   Lemma vmprop_unknown_def : vmprop_unknown ≡
-    λ p_tx p_rx,
-      (∃ (trans' : gmap Word transaction) rxs',
-          transaction_hpool_global_transferred trans' ∗
-          big_sepSS_singleton set_of_vmids i (Φ_t trans') ∗
-          R0 @@ V0 ->r encode_hvc_func(Run) ∗ R1 @@ V0 ->r encode_vmid(i) ∗ (∃ r2, R2 @@ V0 ->r r2) ∗
-          (rx_page i p_rx) ∗
-               (∃ rx_state', rx_state_match i rx_state' ∗
-               match rx_state' with
-               | None => True
-               | Some s => Φ_r i s.2 i
-               end) ∗ (* rx.state'.2 ≠ i *)
+    λ p_tx p_rx, (∃ (trans' : gmap Word transaction) (rxs : gmap VMID (option(Word * VMID))),
+               (* transaction and pagetable entries *)
+               transaction_hpool_global_transferred trans' ∗
+               big_sepSS_singleton set_of_vmids i (Φ_t trans') ∗
+               R0 @@ V0 ->r encode_hvc_func(Run) ∗ R1 @@ V0 ->r encode_vmid(i) ∗ (∃ r2, R2 @@ V0 ->r r2) ∗
+               (* RX *)
+               (rx_page i p_rx) ∗
+               (∀ rs : option (Addr * VMID), ⌜rxs !! i = Some rs⌝ -∗ rx_state_match i rs ∗ Φ_r i rs i) ∗
                (* rx pages for all other VMs *)
-               (rx_states_global (delete i rxs')) ∗
-          VMProp V0 (vmprop_zero p_tx p_rx) (1/2)%Qp)%I.
+               (rx_states_global (delete i rxs)) ∗ ⌜is_total_gmap rxs⌝ ∗
+               (* if i yielding, we give following resources back to pvm *)
+          VMProp V0 (vmprop_zero p_tx p_rx rxs) (1/2)%Qp)%I.
   Proof.
     rewrite /vmprop_unknown //.
     rewrite (fixpoint_unfold vmprop_unknown_pre).
@@ -162,23 +139,22 @@ Section slice.
   Proof. apply _. Qed.
 
   Lemma vmprop_unknown_eq (p_tx p_rx:PID) : vmprop_unknown p_tx p_rx ⊣⊢
-      (∃ (trans' : gmap Word transaction) rxs',
+    (∃ (trans' : gmap Word transaction) (rxs : gmap VMID (option(Word * VMID))),
+               (* transaction and pagetable entries *)
                transaction_hpool_global_transferred trans' ∗
                big_sepSS_singleton set_of_vmids i (Φ_t trans') ∗
                R0 @@ V0 ->r encode_hvc_func(Run) ∗ R1 @@ V0 ->r encode_vmid(i) ∗ (∃ r2, R2 @@ V0 ->r r2) ∗
+               (* RX *)
                (rx_page i p_rx) ∗
-               (∃ rx_state', rx_state_match i rx_state' ∗
-               match rx_state' with
-               | None => True
-               | Some s => Φ_r i s.2 i
-               end) ∗ (* rx.state'.2 ≠ i *)
+               (∀ rs : option (Addr * VMID), ⌜rxs !! i = Some rs⌝ -∗ rx_state_match i rs ∗ Φ_r i rs i) ∗
                (* rx pages for all other VMs *)
-               (rx_states_global (delete i rxs')) ∗
-               VMProp V0 (vmprop_zero p_tx p_rx) (1/2)%Qp)%I.
-    Proof.
-      rewrite /vmprop_unknown.
-      apply (fixpoint_unfold vmprop_unknown_pre).
-    Qed.
+               (rx_states_global (delete i rxs)) ∗ ⌜is_total_gmap rxs⌝ ∗
+               (* if i yielding, we give following resources back to pvm *)
+          VMProp V0 (vmprop_zero p_tx p_rx rxs) (1/2)%Qp)%I.
+  Proof.
+    rewrite /vmprop_unknown.
+    apply (fixpoint_unfold vmprop_unknown_pre).
+  Qed.
 
   End vmprop.
 
@@ -210,17 +186,28 @@ Section logrel_prim.
                 ∗ retrievable_transaction_transferred_slice trans i j
                 ∗ transferred_memory_slice trans i j)%I.
 
-  Definition slice_rx_state (j i: VMID) : iProp Σ :=
-    ∃ p_rx, RX@ j := p_rx ∗ (∃ l,  RX_state{1/2}@j := Some(l, i)) ∗ (∃ mem_rx, memory_page p_rx mem_rx).
+  Definition slice_rx_state (j : VMID) (os : option (Word * VMID)) : iProp Σ :=
+    ∃ p_rx, RX@ j := p_rx ∗ (RX_state{1/2}@j := os) ∗ (∃ mem_rx, memory_page p_rx mem_rx).
 
-  Program Definition interp_access_prim Φ_t Φ_r p_tx p_rx ps_acc trans rxs `{!SliceWf Φ_t}: iPropO Σ:=
+  Definition interp_access_prim (Φ_t : (gmap Addr transaction) -> VMID -> VMID -> iProp Σ)
+    (Φ_r : VMID -> option (Word * VMID)-> VMID -> iProp Σ) (p_tx p_rx :PID) (ps_acc: gset PID) (trans: gmap Word transaction)
+    (rxs : gmap VMID (option (Word * VMID))) `{!SliceWf Φ_t}: iPropO Σ:=
     (
       (* making sure we have enough resources for V0 *)
       ⌜∀ i j trans, (i = V0 ∨ j = V0) -> Φ_t trans i j ⊣⊢ slice_transfer_all trans i j⌝ ∗
-      ⌜∀ i, Φ_r i V0 i ⊣⊢ slice_rx_state i V0 ⌝ ∗
-      ⌜∀ i j, j ≠ i -> Φ_r i V0 j ⊣⊢ True⌝ ∗
-      ⌜∀ i j k k', j ≠ V0 -> Φ_r i j k ⊣⊢ Φ_r i j k'⌝ ∗
-      ⌜∀ i, Φ_r V0 i V0 ⊣⊢ slice_rx_state V0 i ⌝ ∗
+      ⌜∀ i os, (match os with
+                 | None => True
+                 | Some (_,j) => j = V0
+                end) -> Φ_r i os i ⊣⊢ slice_rx_state i os⌝ ∗
+      ⌜∀ i j os, (match os with
+                 | None => True
+                 | Some (_,j) => j = V0
+                end) -> j ≠ i -> Φ_r i os j ⊣⊢ True⌝ ∗
+      ⌜∀ i os k k', (match os with
+                 | None => True
+                 | Some (_,j) => j ≠ V0
+                end) -> Φ_r i os k ⊣⊢ Φ_r i os k'⌝ ∗
+      ⌜∀ i, Φ_r V0 i V0 ⊣⊢ slice_rx_state V0 i⌝ ∗
       let ps_oea := ps_acc ∖ {[p_rx;p_tx]} ∖ (currently_accessible_in_trans_memory_pages V0 trans) in
       (∃ regs, ⌜is_total_gmap regs⌝ ∗ [∗ map] r ↦ w ∈ regs, r @@ V0 ->r w) ∗
       (tx_page V0 p_tx ∗ ∃ mem_tx, memory_page p_tx mem_tx) ∗
@@ -241,7 +228,7 @@ Section logrel_prim.
       [∗ set] i ∈ set_of_vmids ∖ {[V0]}, VMProp (i:VMID) (vmprop_unknown i Φ_t Φ_r p_tx p_rx) (1/2)%Qp
     )%I.
 
-  Program Definition interp_execute_prim: iPropO Σ :=
+  Definition interp_execute_prim: iPropO Σ :=
     WP ExecI @ V0 {{(λ _, True )}}%I.
 
 End logrel_prim.
